theories/closed_async.v
@@ -1,0 +1,323 @@
+From iris.proofmode Require Import tactics.
+From iris.base_logic.lib Require Import invariants.
+From iris.algebra Require Import agree auth.
+From esop Require Import overlap delayed specification typetranslation types corecalculus oneshot.
+From stdpp Require Import gmap coPset.
+
+Section Theory.
+  Context `{allG Σ}.
+  (** Closure: Async operations *)
+  Ltac intro_equiv x := f_equiv; intro x.
+  Local Open Scope I.
+  
+  Lemma closed_post (Γ: env) (η: hexpr) e e' A (τ: type) (η': hexpr) ξ
+        (ξ_fresh_Γ: ξ ∉ names Γ) (ξ_fresh_η: ξ ∉ names η) (ξ_fresh_A: ξ ∉ A)
+        (ξ_fresh_τ: ξ ∉ names τ) (ξ_fresh_η': ξ ∉ names η'):
+    delayed_typed Γ η e e' A τ η' -∗
+                  delayed_typed Γ η (Post e) (Post e') {[ξ]} (ttask ξ A τ) (hwait ξ A η').
+  Proof.
+    iIntros "del".
+    iIntros (D N σ) "pre"; cbn [subst].
+    (* Allocate ghost state *)
+    iApply fupd_wp.
+    iMod (own_alloc (@unset conn_mapC)) as (γD) "ownD"; first done.
+    iMod (own_alloc (@unset name_mapC)) as (γN) "ownN"; first done.
+    set (T := TaskData e' Γ η η' A D γD γN).
+    set (promise_body t x := int_i_promise_body int_s_type int_s_heap N A τ (int_i_type τ) t x).
+    set (wait_body t x := int_i_wait_body η' (int_i_heap η') A N t x).
+    iAssert (∀ t, task_agree t T -∗ WP subst (of_val <$> σ) e
+                             {{ x, promise_body t x ∗ wait_body t x }})
+            with "[ownD ownN del pre]" as "wp".
+    { iSpecialize ("del" with "pre").
+      iIntros (t) "#agree_t".
+      iApply wp_fupd.
+      iApply (wp_wand with "del").
+      iIntros (v) "H".
+      iDestruct "H" as (N' D' d') "[eqs [ty [#sim heap]]]".
+      iMod (own_update _ _ (agreed D') with "ownD") as "#ownD"; first apply oneshot_update.
+      iMod (own_update _ _ (agreed (N': leibnizC name_map)) with "ownN") as "#ownN";
+        first apply oneshot_update.
+      iModIntro.
+      iDestruct "eqs" as %[eqN eqd].
+      iSplitR "heap".
+      - iExists T, D', N'.
+        iSplit.
+        { repeat iSplit; auto. }
+        rewrite /ip_impl /ip_sim.
+        iSplitL "ty".
+        { iExists d'; iSplit; last done.
+          iPureIntro.
+          assert (of_gset (names τ ∖ A) ⊆ not_new A).
+          { intro; rewrite elem_of_of_gset elem_of_not_new elem_of_difference; tauto. }
+          repeat split; auto.
+          all: apply overlap_cast; by eapply overlap_mono. }
+        iAlways.
+        iSplit; first done.
+        iExact "sim".
+      - iExists T, D', N'; iFrame.
+        repeat iSplit; auto.
+        iPureIntro.
+        apply overlap_cast, (overlap_sub (not_new A)); last done.
+        intro; rewrite elem_of_of_gset elem_of_difference elem_of_not_new; tauto. }
+    iPoseProof (wp_post ⊤ with "wp") as "wp".
+    iModIntro.
+    iApply wp_fupd.
+    iApply (wp_wand with "wp").
+    iIntros (v) "H".
+    iDestruct "H" as (t) "[% [wait #t_agree]]"; subst.
+    iPoseProof (wait_split with "wait") as "waits".
+    iPoseProof (fupd_mask_mono _ ⊤ with "waits") as "waits"; first auto.
+    iMod "waits" as "[promise wait]".      
+    iMod (inv_alloc promiseN with "promise") as "promise".
+    iAssert (int_i_type (Promise(ξ,A) τ) Cunit (<[ξ:=Task t]>N) (Ctid t))
+    with "[promise]" as "promise".
+    { cbn; iExists t; iSplit.
+      - rewrite !lookup_insert; auto.
+      - iApply (inv_Proper with "promise").
+        apply wait_Proper; intros t' v'.
+        rewrite /promise_body /int_i_promise_body /ip_impl.
+        intro_equiv U; intro_equiv D'; intro_equiv N'.
+        do 2 f_equiv; intro_equiv d.
+        do 3 f_equiv.
+        apply (overlap_iff (names τ ∖ A)); first done.
+        intros ξ' inξ'.
+        rewrite lookup_insert_ne; first done.
+        clear -inξ' ξ_fresh_τ; set_solver. }
+    iAssert (int_i_heap (Wait(ξ,A) η') (<[name ξ:=VConst (Ctid t)]>(<[RET:=VConst Cunit]>∅))
+                        (<[ξ:=Task t]>N))
+    with "[wait]" as "wait".
+    { cbn; iExists t.
+      rewrite !lookup_insert; iSplit; auto.
+      iApply (wait_Proper with "wait"); intros t' v.
+      rewrite /wait_body /int_i_wait_body.
+      intro_equiv U; intro_equiv D'; intro_equiv N'.
+      do 4 f_equiv.
+      intro ξ'; rewrite elem_of_difference => [[inξ' notinξ']].
+      rewrite lookup_insert_ne; first done.
+      intros <-; contradiction. }
+    iModIntro.
+    iExists (<[ξ:=Task t]>N), (<[name ξ:=VConst (Ctid t)]>(<[RET:=VConst Cunit]>∅)), (VConst Cunit).
+    iFrame.
+    iSplit.
+    { rewrite lookup_insert_ne ?lookup_insert; last discriminate.
+      iPureIntro; split; last done.
+      intros ξ'.
+      rewrite elem_of_not_new not_elem_of_singleton => [neq].
+      rewrite lookup_insert_ne; done. }
+    clear σ N promise_body wait_body.
+    iAlways.
+    iIntros (N σ p K) "#ctx [env pre] move"; cbn -[difference].
+    iMod (simulate_post ⊤ _ p K N with "ctx move") as (p') "[move [move' [#agree neq]]]"; auto.
+    iModIntro.
+    iDestruct "pre" as (n) "pre".
+    iExists (Ctid p'); iFrame.
+    iExists (VConst Cunit), (<[ξ:=Task p']>N).
+    iSplit.
+    { iDestruct "neq" as %neq; iPureIntro.
+      split.
+      - intro ξ'; rewrite elem_of_not_new not_elem_of_singleton => [neq'].
+        rewrite lookup_insert_ne; done.
+      - rewrite lookup_insert_ne ?lookup_insert; done. }
+    iSplit.
+    { rewrite /int_s_promise.
+      iExists p', N.
+      iSplit; first done.
+      rewrite lookup_insert.
+      iPureIntro; repeat split; auto.
+      intros ξ'.
+      rewrite elem_of_difference => [[inξ' notinξ']].
+      rewrite lookup_insert_ne; first done.
+      intros <-; contradiction. }
+    iExists (S n); rewrite /= /int_s_wait.
+    iExists t, p', T, σ.
+    iSplit.
+    { iPureIntro; rewrite !lookup_insert; auto. }
+    iSplit; auto.
+    iFrame.
+    iExists N; iFrame.
+    iSplit; auto.
+    { iPureIntro.
+      intro ξ'.
+      rewrite elem_of_difference => [[inξ' notinξ']].
+      rewrite lookup_insert_ne; first done.
+      intros <-; contradiction. }
+    Unshelve. auto.
+  Qed.
+
+  Instance wait_proper t:
+    Proper (pointwise_relation _ (pointwise_relation _ (≡)) ==> (⊣⊢)) (wait t).
+  Proof.
+    intros ϕ ϕ' eqϕ.
+    rewrite equiv_dist => [n].
+    apply: wait_nonexpansive => [t' v].
+    rewrite eqϕ; done.
+  Qed.
+
+  Lemma task_agree_eq t U U': task_agree t U -∗ task_agree t U' -∗ ⌜U = U'⌝.
+  Proof.
+    iIntros "ag ag'".
+    iPoseProof (own_valid_2 with "ag ag'") as "valid".
+    rewrite uPred.discrete_valid.
+    rewrite gmap.op_singleton gmap.singleton_valid.
+    iDestruct "valid" as %->%agree.agree_op_invL'; auto.
+  Qed.
+
+  
+  Lemma agreed_equiv {A: ofeT} {Adiscr: Discrete A}
+        {inA: inG Σ (oneshotR A)} γ (x x': A):
+    (own γ (agreed x) -∗ own γ (agreed x') -∗ ⌜x ≡ x'⌝).
+  Proof.
+    iIntros "ag ag'".
+    iPoseProof (own_valid_2 with "ag ag'") as "valid".
+    rewrite uPred.discrete_valid /agreed csum.Cinr_op.
+    iDestruct "valid" as %?%agree.agree_op_inv'; auto.
+  Qed.
+
+  Lemma agreed_eq {A: Type}
+        {inA: inG Σ (oneshotR (leibnizC A))} γ (x x': A):
+    (own γ (agreed (x: leibnizC A)) -∗ own γ (agreed (x': leibnizC A)) -∗ ⌜x = x'⌝).
+  Proof. iApply (@agreed_equiv (leibnizC A) _ inA γ x x'). Qed.
+
+  Lemma spec_task_agree_eq t A A': spec_task_agree t A -∗ spec_task_agree t A' -∗ ⌜A = A'⌝.
+  Proof.
+    iIntros "ag ag'".
+    rewrite /spec_task_agree.
+    iPoseProof (own_valid_2 with "ag ag'") as "valid".
+    rewrite uPred.discrete_valid.
+    rewrite -auth_frag_op gmap.op_singleton.
+    iDestruct "valid" as %<-%gmap.singleton_valid%agree_op_invL'; auto.
+  Qed.
+  
+  Lemma closed_wait (x: string) ξ A (τ: type) (η: hexpr)
+        (ξ_not_in_τ: ξ ∉ names τ) (ξ_not_in_η: ξ ∉ names η):
+    delayed_typed (<[x:=ttask ξ A τ]>∅) (hwait ξ A η) (Wait x) (Wait x) A τ η.
+  Proof.
+    iIntros (D N σ) "[[env_names env] pre]".
+    iDestruct "env_names" as %[domσ domD].
+    assert (is_Some (σ !! x)) as [v val_x].
+    { apply domσ; rewrite lookup_insert; eauto. }
+    assert (is_Some (D !! var x)) as [d conn_x].
+    { apply domD; rewrite lookup_insert; eauto. }
+    iDestruct ("env" $! x _ v d with "[]") as "#promise".
+    { rewrite /int_env_data lookup_insert; eauto. }
+    rewrite /= lookup_fmap val_x /=.
+    iDestruct "promise" as (t) "[eqs promise]".
+    iDestruct "eqs" as %[taskξ ->].
+    iApply fupd_wp.
+    iInv promiseN as "promisewait" "close".
+    iPoseProof (wait_split_later with "[promisewait]") as "split".
+    { iNext.
+      iApply (wait_proper t with "promisewait").
+      iIntros (t' v); iSplit.
+      - iIntros "[pb _]"; iExact "pb".
+      - rewrite /int_i_promise_body.
+        iIntros "#pre".
+        iSplit; iExact "pre". }
+    iPoseProof (fupd_mask_mono _ (⊤ ∖ ↑promiseN) with "split") as "split"; first solve_ndisj.
+    iMod "split" as "[promisewait pw']".
+    iMod ("close" with "pw'") as "_".
+    iDestruct "pre" as (t') "[names pre]".
+    rewrite taskξ.
+    iDestruct "names" as %[[=<-] taskξD].
+    iPoseProof (wait_combine_later with "[$pre $promisewait]") as "wait".
+    iPoseProof (fupd_mask_mono _ ⊤ with "wait") as "wait"; first solve_ndisj.
+    iMod "wait" as "wait".
+    iModIntro.
+    iPoseProof (wp_wait with "wait") as "wp".
+    iApply (wp_wand with "wp").
+    iIntros (v) "[wb pb]".
+    iDestruct "wb" as (U D' N') "[[#agreeU [#agreeD' #agreeN']] [ovη post]]".
+    iDestruct "ovη" as %ovη.
+    iDestruct "pb" as (U' D'' N'') "[[agreeU' [agreeD'' agreeN'']] [H #sim]]".
+    iDestruct "H" as (d') "[names type]".
+    iDestruct "names" as %[eqd' ovτ].
+    iDestruct (task_agree_eq with "agreeU agreeU'") as %<-; iClear "agreeU'".
+    iDestruct (agreed_eq (A := conn_map) with "agreeD' agreeD''") as %<-; iClear "agreeD''".
+    iDestruct (agreed_eq (A := name_map) with "agreeN' agreeN''") as %<-; iClear "agreeN''".
+    iExists (N' ~[A]~> N), D', d'.
+    repeat iSplit.
+    { iPureIntro.
+      intro ξ'.
+      rewrite elem_of_not_new => [notinξ'].
+      rewrite lookup_merge_along_not_in; done. }
+    { done. }
+    { iApply (int_i_type_local with "type").
+      1,3: done.
+      intros ξ' inξ'.
+      destruct (decide (ξ' ∈ A)) as [case|case].
+      - by rewrite lookup_merge_along_in.
+      - rewrite lookup_merge_along_not_in; last done.
+        rewrite (ovτ ξ') ?elem_of_difference; auto. }
+    all: cycle 1.
+    { iApply (int_i_heap_local with "post").
+      { done. }
+      intros ξ' inξ'.
+      destruct (decide (ξ' ∈ A)) as [case|case].
+      - by rewrite lookup_merge_along_in.
+      - rewrite lookup_merge_along_not_in; last done.
+        rewrite (ovη ξ') ?elem_of_difference; auto. }
+    iClear "post type promise agreeN'"; iAlways.
+    clear N N' ovη ovτ taskξ σ domσ val_x v.
+    iIntros (N σ p K) "#ctx [[env_names promise] wait] move".
+    iDestruct "env_names" as %[domσ _].
+    assert (is_Some (σ !! x)) as [v val_x].
+    { apply domσ; rewrite lookup_insert; eauto. }    
+    iSpecialize ("promise" $! x (ttask ξ A τ) v d with "[]").
+    { rewrite /int_env_data lookup_insert; auto. }
+    iDestruct "sim" as "[% sim]"; subst A.
+    iDestruct "promise" as (ts Npre) "[agreePre names]".
+    iDestruct "names" as %[taskξ [Npreτ ->]].
+    iDestruct "wait" as ([|n]) "wait"; cbn [int_s_heap int_s_heap_rec int_s_heap_approx].
+    all: iDestruct "wait" as (ti' ts' U' σ') "[names [agreeU' [move' pre]]]".
+    all: iDestruct "pre" as (Npre') "[env [pre [agreeNpre' Npreη]]]".
+    { iDestruct "pre" as "[]". }
+    rewrite taskξ taskξD.
+    iDestruct "names" as %[[=<-] [[=<-] [<- ->]]].
+    iDestruct (task_agree_eq with "agreeU agreeU'") as %<-; iClear "agreeU'".
+    iDestruct (spec_task_agree_eq with "agreePre agreeNpre'") as %<-.
+    iSpecialize ("sim" $! Npre σ' ts [] with "ctx [$env pre]").
+    { by iExists n. }
+    iDestruct "Npreη" as %Npreη; iClear "agreeNpre' agreePre agreeU agreeD'".
+    rewrite /= lookup_fmap val_x /=.
+    iMod (simulate_wait_schedule with "ctx move move'") as "[move move']"; first auto.
+    iMod ("sim" with "move'") as (v) "[post move']".
+    iMod (simulate_done_schedule with "ctx move' move") as "[move' move]"; first auto.
+    { apply to_of_val. }
+    iAssert (⌜p ≠ ts⌝) with "[move move']" as %neqp.
+    { iDestruct "move" as "[move _]".
+      iPoseProof (own_valid_2 with "move move'") as "valid".
+      rewrite /task_runnable /task_done -auth_frag_op uPred.discrete_valid.
+      iDestruct "valid" as %valid.
+      iPureIntro; intros <-.
+      rewrite gmap.op_singleton in valid.
+      rewrite auth_valid_eq /= gmap.singleton_valid in valid * => [[]]. }
+    iMod (simulate_wait_done with "ctx move move'") as "[move _]"; auto.
+    iExists v; iFrame.
+    iModIntro.
+    iDestruct "post" as (ds' Ns') "[names [type heap]]".
+    iDestruct "names" as %[Npre' eqD'].
+    iExists ds', (Ns' ~[td_alloc U]~> N).
+    iSplit.
+    { iPureIntro; split; auto.
+      intros ξ'.
+      rewrite elem_of_not_new => [notinξ'].
+      rewrite lookup_merge_along_not_in; done. }
+    iSplit.
+    - iApply (int_s_type_local with "type").
+      1,3: done.
+      intros ξ' inξ'.
+      destruct (decide (ξ' ∈ td_alloc U)) as [case|case].
+      { by rewrite lookup_merge_along_in. }
+      rewrite lookup_merge_along_not_in; last done.
+      rewrite -(Npreτ ξ') ?elem_of_difference; last done.
+      rewrite (Npre' ξ') ?elem_of_not_new; done.
+    - iApply (int_s_heap_local with "heap").
+      1: done.
+      intros ξ' inξ'.
+      destruct (decide (ξ' ∈ td_alloc U)) as [case|case].
+      { by rewrite lookup_merge_along_in. }
+      rewrite lookup_merge_along_not_in; last done.
+      rewrite -(Npreη ξ') ?elem_of_difference; last done.
+      rewrite (Npre' ξ') ?elem_of_not_new; done.
+  Qed.
+End Theory.
